src/LoopfreeWF.v
@@ -1,0 +1,43 @@
+Require Import CpdtTactics.
+Require Import Closures.
+
+Set Implicit Arguments.
+
+Section LOOPFREE.
+
+Variable A: Type.
+Variable step: A -> A -> Prop.
+Variable WF: well_founded step.
+Hint Resolve WF.
+
+Theorem wf_norefl:
+  forall (a:A),
+  ~step a a.
+Proof.
+  unfold not; intros; assert (Acc step a); auto.
+  induction H0; eapply H1; apply H.
+Qed.
+
+Lemma wf_loopfree':
+  forall (x y:A),
+  step x y -> star step y x -> False.
+Proof.
+  unfold not; intro x; assert (Acc step x); auto.
+  induction H; intros.
+  inversion H2; subst.
+  - exact (wf_norefl H1).
+  - destruct (star_last H3 H4).
+    apply H0 with (y:=x0) (y0:=x); intuition.
+    eapply star_step; eauto.
+Qed.
+
+Lemma wf_loopfree:
+  forall (x y:A),
+  star step x y -> star step y x -> x = y.
+Proof.
+  intros; inversion H; auto; subst.
+  assert (star step s2 x). eapply star_trans; eauto.
+  destruct (wf_loopfree' H1 H3).
+Qed.
+
+End LOOPFREE.
